Added hoare_heap_write

Hoare.v
@@ -7,6 +7,10 @@ Require Import Coq.omega.Omega.
 Require Import Imp.
 Require Import Maps.
 
+Definition X : id := Id 0.
+Definition Y : id := Id 1.
+Definition Z : id := Id 2.
+
 
 (* ################################################################# *)
 (** * Assertions *)
@@ -15,7 +19,7 @@ Require Import Maps.
 Definition Assertion := heap -> valuation -> Prop.
 
 Definition assert_implies (P Q : Assertion) : Prop :=
-  forall (h h' : heap) (v v' : valuation), P h v -> Q h' v'.
+  forall (h : heap) (v : valuation), P h v -> Q h v.
 
 Notation "P ->> Q" := (assert_implies P Q)
                       (at level 80) : hoare_spec_scope.
@@ -30,7 +34,7 @@ Notation "P <<->> Q" :=
 Definition hoare_triple
            (P:Assertion) (c:com) (Q:Assertion) : Prop :=
   forall (h h' : heap) (v v' : valuation),
-     ceval c h v h' v'  ->
+     ceval h v c h' v'  ->
      P h v  ->
      Q h' v'.
 
@@ -69,7 +73,7 @@ Proof.
 
 Definition assn_sub X a P : Assertion :=
   fun (h : heap) (v : valuation) =>
-    P h (t_update v X (aeval v h a)).
+    P h (t_update v X (aeval h v a)).
 
 Notation "P [ X |-> a ]" := (assn_sub X a P) (at level 10).
 
@@ -81,64 +85,10 @@ Proof.
   inversion H. subst.
   unfold assn_sub in H0. apply H0.  Qed.
 
-(** Here's a first formal proof using this rule. *)
-
-Example assn_sub_example :
-  {{(fun h v => v X = 3) [X |-> ANum 3]}}
-  (X ::= (ANum 3))
-  {{fun h v => v X = 3}}.
-Proof.
-  apply hoare_asgn.  Qed.
-
-Example assn_sub_ex1 :
-  {{(fun h v =>  v X <= 5) [X |-> APlus (AId X) (ANum 1)] }}
-     (X ::= APlus (AId X) (ANum 1))
-     {{(fun h v =>  v X <= 5 )}}.
-Proof.
-  apply hoare_asgn. Qed.
-
-Example assn_sub_ex2 :
-  {{(fun h v =>  (0 <= v X /\ v X <= 5)) [X |-> ANum 3]}}
-  X ::= ANum 3
-  {{ (fun h v => (0 <= v X /\ v X <= 5)) }}.
-Proof.
-  apply hoare_asgn. Qed.
-  
-
 (* ================================================================= *)
 (** ** Consequence *)
 
-(** Sometimes the preconditions and postconditions we get from the
-    Hoare rules won't quite be the ones we want in the particular
-    situation at hand -- they may be logically equivalent but have a
-    different syntactic form that fails to unify with the goal we are
-    trying to prove, or they actually may be logically weaker (for
-    preconditions) or stronger (for postconditions) than what we need.
-    For instance, while
-
-      {{(X = 3) [X |-> 3]}} X ::= 3 {{X = 3}},
-
-    follows directly from the assignment rule,
-
-      {{True}} X ::= 3 {{X = 3}}
-
-    does not.  This triple is valid, but it is not an instance of
-    [hoare_asgn] because [True] and [(X = 3) [X |-> 3]] are not
-    syntactically equal assertions.  However, they are logically
-    equivalent, so if one triple is valid, then the other must
-    certainly be as well.  We can capture this observation with the
-    following rule:
-
-                {{P'}} c {{Q}}
-                  P <<->> P'
-         -----------------------------   (hoare_consequence_pre_equiv)
-                {{P}} c {{Q}}
-
-    Taking this line of thought a bit further, we can see that
-    strengthening the precondition or weakening the postcondition of a
-    valid triple always produces another valid triple. This
-    observation is captured by two _Rules of Consequence_.
-
+(** 
                 {{P'}} c {{Q}}
                    P ->> P'
          -----------------------------   (hoare_consequence_pre)
@@ -157,43 +107,23 @@ Theorem hoare_consequence_pre : forall (P P' Q : Assertion) c,
   P ->> P' ->
   {{P}} c {{Q}}.
 Proof.
-  intros P P' Q c Hhoare Himp.
-  intros st st' Hc HP. apply (Hhoare st st').
-  assumption. apply Himp. assumption. Qed.
+  intros P P' Q c Hhoare Himp. unfold hoare_triple.
+  intros. apply (Hhoare h h' v v').
+  assumption. unfold assert_implies in Himp. apply Himp. assumption. Qed.
 
 Theorem hoare_consequence_post : forall (P Q Q' : Assertion) c,
   {{P}} c {{Q'}} ->
   Q' ->> Q ->
   {{P}} c {{Q}}.
 Proof.
-  intros P Q Q' c Hhoare Himp.
-  intros st st' Hc HP.
+  intros P Q Q' c Hhoare Himp. unfold hoare_triple.
+  intros.
+  unfold assert_implies in Himp.
   apply Himp.
-  apply (Hhoare st st').
+  apply (Hhoare h h' v v').
   assumption. assumption. Qed.
 
-(** For example, we can use the first consequence rule like this:
-
-                {{ True }} ->>
-                {{ 1 = 1 }}
-    X ::= 1
-                {{ X = 1 }}
-
-    Or, formally... *)
-
-Example hoare_asgn_example1 :
-  {{fun st => True}} (X ::= (ANum 1)) {{fun st => st X = 1}}.
-Proof.
-  apply hoare_consequence_pre
-    with (P' := (fun st => st X = 1) [X |-> ANum 1]).
-  apply hoare_asgn.
-  intros st H. unfold assn_sub, t_update. simpl. reflexivity.
-Qed.
-
-(** Finally, for convenience in some proofs, we can state a combined
-    rule of consequence that allows us to vary both the precondition
-    and the postcondition at the same time.
-
+(** 
                 {{P'}} c {{Q'}}
                    P ->> P'
                    Q' ->> Q
@@ -208,133 +138,10 @@ Theorem hoare_consequence : forall (P P' Q Q' : Assertion) c,
   {{P}} c {{Q}}.
 Proof.
   intros P P' Q Q' c Hht HPP' HQ'Q.
+  Check hoare_consequence_pre.
   apply hoare_consequence_pre with (P' := P').
   apply hoare_consequence_post with (Q' := Q').
   assumption. assumption. assumption.  Qed.
-
-(* ================================================================= *)
-(** ** Digression: The [eapply] Tactic *)
-
-(** This is a good moment to introduce another convenient feature of
-    Coq.  We had to write "[with (P' := ...)]" explicitly in the proof
-    of [hoare_asgn_example1] and [hoare_consequence] above, to make
-    sure that all of the metavariables in the premises to the
-    [hoare_consequence_pre] rule would be set to specific
-    values.  (Since [P'] doesn't appear in the conclusion of
-    [hoare_consequence_pre], the process of unifying the conclusion
-    with the current goal doesn't constrain [P'] to a specific
-    assertion.)
-
-    This is annoying, both because the assertion is a bit long and
-    also because, in [hoare_asgn_example1], the very next thing we are
-    going to do -- applying the [hoare_asgn] rule -- will tell us
-    exactly what it should be!  We can use [eapply] instead of [apply]
-    to tell Coq, essentially, "Be patient: The missing part is going
-    to be filled in later in the proof." *)
-
-Example hoare_asgn_example1' :
-  {{fun st => True}}
-  (X ::= (ANum 1))
-  {{fun st => st X = 1}}.
-Proof.
-  eapply hoare_consequence_pre.
-  apply hoare_asgn.
-  intros st H.  reflexivity.  Qed.
-
-(** In general, [eapply H] tactic works just like [apply H] except
-    that, instead of failing if unifying the goal with the conclusion
-    of [H] does not determine how to instantiate all of the variables
-    appearing in the premises of [H], [eapply H] will replace these
-    variables with _existential variables_ (written [?nnn]), which
-    function as placeholders for expressions that will be
-    determined (by further unification) later in the proof. *)
-
-(** In order for [Qed] to succeed, all existential variables need to
-    be determined by the end of the proof. Otherwise Coq
-    will (rightly) refuse to accept the proof. Remember that the Coq
-    tactics build proof objects, and proof objects containing
-    existential variables are not complete. *)
-
-Lemma silly1 : forall (P : nat -> nat -> Prop) (Q : nat -> Prop),
-  (forall x y : nat, P x y) ->
-  (forall x y : nat, P x y -> Q x) ->
-  Q 42.
-Proof.
-  intros P Q HP HQ. eapply HQ. apply HP.
-
-(** Coq gives a warning after [apply HP].  (The warnings look
-    different between Coq 8.4 and Coq 8.5.  In 8.4, the warning says
-    "No more subgoals but non-instantiated existential variables."  In
-    8.5, it says "All the remaining goals are on the shelf," meaning
-    that we've finished all our top-level proof obligations but along
-    the way we've put some aside to be done later, and we have not
-    finished those.)  Trying to close the proof with [Qed] gives an
-    error. *)
-
-Abort.
-
-(** An additional constraint is that existential variables cannot be
-    instantiated with terms containing ordinary variables that did not
-    exist at the time the existential variable was created.  (The
-    reason for this technical restriction is that allowing such
-    instantiation would lead to inconsistency of Coq's logic.) *)
-
-Lemma silly2 :
-  forall (P : nat -> nat -> Prop) (Q : nat -> Prop),
-  (exists y, P 42 y) ->
-  (forall x y : nat, P x y -> Q x) ->
-  Q 42.
-Proof.
-  intros P Q HP HQ. eapply HQ. destruct HP as [y HP'].
-
-(** Doing [apply HP'] above fails with the following error:
-
-     Error: Impossible to unify "?175" with "y".
-
-    In this case there is an easy fix: doing [destruct HP] _before_
-    doing [eapply HQ]. *)
-
-Abort.
-
-Lemma silly2_fixed :
-  forall (P : nat -> nat -> Prop) (Q : nat -> Prop),
-  (exists y, P 42 y) ->
-  (forall x y : nat, P x y -> Q x) ->
-  Q 42.
-Proof.
-  intros P Q HP HQ. destruct HP as [y HP'].
-  eapply HQ. apply HP'.
-Qed.
-
-(** The [apply HP'] in the last step unifies the existential variable
-    in the goal with the variable [y].
-
-    Note that the [assumption] tactic doesn't work in this case, since
-    it cannot handle existential variables.  However, Coq also
-    provides an [eassumption] tactic that solves the goal if one of
-    the premises matches the goal up to instantiations of existential
-    variables. We can use it instead of [apply HP'] if we like. *)
-
-Lemma silly2_eassumption : forall (P : nat -> nat -> Prop) (Q : nat -> Prop),
-  (exists y, P 42 y) ->
-  (forall x y : nat, P x y -> Q x) ->
-  Q 42.
-Proof.
-  intros P Q HP HQ. destruct HP as [y HP']. eapply HQ. eassumption.
-Qed.
-
-(** **** Exercise: 2 stars (hoare_asgn_examples_2)  *)
-(** Translate these informal Hoare triples...
-
-       {{ X + 1 <= 5 }}  X ::= X + 1  {{ X <= 5 }}
-       {{ 0 <= 3 /\ 3 <= 5 }}  X ::= 3  {{ 0 <= X /\ X <= 5 }}
-
-   ...into formal statements (name them [assn_sub_ex1'] and 
-   [assn_sub_ex2']) and use [hoare_asgn] and [hoare_consequence_pre] 
-   to prove them. *)
-
-(* FILL IN HERE *)
-(** [] *)
 
 (* ================================================================= *)
 (** ** Skip *)
@@ -349,18 +156,13 @@ Qed.
 Theorem hoare_skip : forall P,
      {{P}} SKIP {{P}}.
 Proof.
-  intros P st st' H HP. inversion H. subst.
+  unfold hoare_triple. intros. inversion H. subst.
   assumption.  Qed.
 
 (* ================================================================= *)
 (** ** Sequencing *)
 
-(** More interestingly, if the command [c1] takes any state where
-    [P] holds to a state where [Q] holds, and if [c2] takes any
-    state where [Q] holds to one where [R] holds, then doing [c1]
-    followed by [c2] will take any state where [P] holds to one
-    where [R] holds:
-
+(** 
         {{ P }} c1 {{ Q }}
         {{ Q }} c2 {{ R }}
        ---------------------  (hoare_seq)
@@ -372,403 +174,63 @@ Theorem hoare_seq : forall P Q R c1 c2,
      {{P}} c1 {{Q}} ->
      {{P}} c1;;c2 {{R}}.
 Proof.
-  intros P Q R c1 c2 H1 H2 st st' H12 Pre.
-  inversion H12; subst.
-  apply (H1 st'0 st'); try assumption.
-  apply (H2 st st'0); assumption. Qed.
-
-(** Note that, in the formal rule [hoare_seq], the premises are
-    given in backwards order ([c2] before [c1]).  This matches the
-    natural flow of information in many of the situations where we'll
-    use the rule, since the natural way to construct a Hoare-logic
-    proof is to begin at the end of the program (with the final
-    postcondition) and push postconditions backwards through commands
-    until we reach the beginning. *)
-
-(** Informally, a nice way of displaying a proof using the sequencing
-    rule is as a "decorated program" where the intermediate assertion
-    [Q] is written between [c1] and [c2]:
-
-      {{ a = n }}
-    X ::= a;;
-      {{ X = n }}    <---- decoration for Q
-    SKIP
-      {{ X = n }}
-*)
-
-(** Here's an example of a program involving both assignment and
-    sequencing. *)
-
-Example hoare_asgn_example3 : forall a n,
-  {{fun st => aeval st a = n}}
-  (X ::= a;; SKIP)
-  {{fun st => st X = n}}.
-Proof.
-  intros a n. eapply hoare_seq.
-  - (* right part of seq *)
-    apply hoare_skip.
-  - (* left part of seq *)
-    eapply hoare_consequence_pre. apply hoare_asgn.
-    intros st H. subst. reflexivity. 
+  unfold hoare_triple. intros.
+  inversion H1. subst.
+  apply H with h2 v2. try assumption.
+  apply H0 with h v. assumption. assumption.
 Qed.
-
-(** We typically use [hoare_seq] in conjunction with
-    [hoare_consequence_pre] and the [eapply] tactic, as in this
-    example. *)
-
-(** **** Exercise: 2 stars (hoare_asgn_example4)  *)
-(** Translate this "decorated program" into a formal proof:
-
-                   {{ True }} ->>
-                   {{ 1 = 1 }}
-    X ::= 1;;
-                   {{ X = 1 }} ->>
-                   {{ X = 1 /\ 2 = 2 }}
-    Y ::= 2
-                   {{ X = 1 /\ Y = 2 }}
-*)
-
-Example hoare_asgn_example4 :
-  {{fun st => True}} (X ::= (ANum 1);; Y ::= (ANum 2))
-  {{fun st => st X = 1 /\ st Y = 2}}.
-Proof.
-  (* FILL IN HERE *) Admitted.
-(** [] *)
-
-(** **** Exercise: 3 stars (swap_exercise)  *)
-(** Write an Imp program [c] that swaps the values of [X] and [Y] and
-    show that it satisfies the following specification:
-
-      {{X <= Y}} c {{Y <= X}}
-*)
-
-Definition swap_program : com 
-  (* REPLACE THIS LINE WITH   := _your_definition_ . *) . Admitted.
-
-Theorem swap_exercise :
-  {{fun st => st X <= st Y}}
-  swap_program
-  {{fun st => st Y <= st X}}.
-Proof.
-  (* FILL IN HERE *) Admitted.
-(** [] *)
-
-(** **** Exercise: 3 stars (hoarestate1)  *)
-(** Explain why the following proposition can't be proven:
-
-      forall (a : aexp) (n : nat),
-         {{fun st => aeval st a = n}}
-         (X ::= (ANum 3);; Y ::= a)
-         {{fun st => st Y = n}}.
-*)
-
-(* FILL IN HERE *)
-(** [] *)
 
 (* ================================================================= *)
 (** ** Conditionals *)
 
-(** What sort of rule do we want for reasoning about conditional
-    commands?  
-
-    Certainly, if the same assertion [Q] holds after executing 
-    either of the branches, then it holds after the whole conditional.  
-    So we might be tempted to write:
-
-              {{P}} c1 {{Q}}
-              {{P}} c2 {{Q}}
-      --------------------------------
-      {{P}} IFB b THEN c1 ELSE c2 {{Q}}
-
-   However, this is rather weak. For example, using this rule,
-   we cannot show 
-
-     {{ True }}
-     IFB X == 0
-     THEN Y ::= 2
-     ELSE Y ::= X + 1
-     FI
-     {{ X <= Y }}
-
-   since the rule tells us nothing about the state in which the
-   assignments take place in the "then" and "else" branches. *)
-
-(** Fortunately, we can say something more precise.  In the
-    "then" branch, we know that the boolean expression [b] evaluates to
-    [true], and in the "else" branch, we know it evaluates to [false].
-    Making this information available in the premises of the rule gives
-    us more information to work with when reasoning about the behavior
-    of [c1] and [c2] (i.e., the reasons why they establish the
-    postcondition [Q]). *)
-(**
+(** 
 
               {{P /\  b}} c1 {{Q}}
               {{P /\ ~b}} c2 {{Q}}
       ------------------------------------  (hoare_if)
       {{P}} IFB b THEN c1 ELSE c2 FI {{Q}}
-*)
-
-(** To interpret this rule formally, we need to do a little work.
-    Strictly speaking, the assertion we've written, [P /\ b], is the
-    conjunction of an assertion and a boolean expression -- i.e., it
-    doesn't typecheck.  To fix this, we need a way of formally
-    "lifting" any bexp [b] to an assertion.  We'll write [bassn b] for
-    the assertion "the boolean expression [b] evaluates to [true] (in
-    the given state)." *)
+ *)
 
 Definition bassn b : Assertion :=
-  fun st => (beval st b = true).
+  fun h v => (beval h v b = true).
 
 (** A couple of useful facts about [bassn]: *)
 
-Lemma bexp_eval_true : forall b st,
-  beval st b = true -> (bassn b) st.
+Lemma bexp_eval_true : forall b h v,
+  beval h v b = true -> (bassn b) h v.
 Proof.
-  intros b st Hbe.
+  intros.
   unfold bassn. assumption.  Qed.
 
-Lemma bexp_eval_false : forall b st,
-  beval st b = false -> ~ ((bassn b) st).
+Lemma bexp_eval_false : forall b h v,
+  beval h v b = false -> ~ ((bassn b) h v).
 Proof.
-  intros b st Hbe contra.
+  intros b h v Hbe contra.
   unfold bassn in contra.
   rewrite -> contra in Hbe. inversion Hbe.  Qed.
 
-(** Now we can formalize the Hoare proof rule for conditionals
-    and prove it correct. *)
-
 Theorem hoare_if : forall P Q b c1 c2,
-  {{fun st => P st /\ bassn b st}} c1 {{Q}} ->
-  {{fun st => P st /\ ~(bassn b st)}} c2 {{Q}} ->
+  {{fun h v => P h v /\ bassn b h v}} c1 {{Q}} ->
+  {{fun h v => P h v /\ ~(bassn b h v)}} c2 {{Q}} ->
   {{P}} (IFB b THEN c1 ELSE c2 FI) {{Q}}.
 Proof.
-  intros P Q b c1 c2 HTrue HFalse st st' HE HP.
+  intros P Q b c1 c2 HTrue HFalse h h' v v' HE HP.
   inversion HE; subst.
   - (* b is true *)
-    apply (HTrue st st').
+    unfold hoare_triple in HTrue.
+    apply (HTrue h h' v v').
       assumption.
       split. assumption.
              apply bexp_eval_true. assumption.
   - (* b is false *)
-    apply (HFalse st st').
+    apply (HFalse h h' v v').
       assumption.
       split. assumption.
              apply bexp_eval_false. assumption. Qed.
 
 (* ----------------------------------------------------------------- *)
-(** *** Example *)
-
-(** Here is a formal proof that the program we used to motivate the
-    rule satisfies the specification we gave. *)
-
-Example if_example :
-    {{fun st => True}}
-  IFB (BEq (AId X) (ANum 0))
-    THEN (Y ::= (ANum 2))
-    ELSE (Y ::= APlus (AId X) (ANum 1))
-  FI
-    {{fun st => st X <= st Y}}.
-Proof.
-  (* WORKED IN CLASS *)
-  apply hoare_if.
-  - (* Then *)
-    eapply hoare_consequence_pre. apply hoare_asgn.
-    unfold bassn, assn_sub, t_update, assert_implies.
-    simpl. intros st [_ H].
-    apply beq_nat_true in H.
-    rewrite H. omega.
-  - (* Else *)
-    eapply hoare_consequence_pre. apply hoare_asgn.
-    unfold assn_sub, t_update, assert_implies.
-    simpl; intros st _. omega.
-Qed.
-
-(** **** Exercise: 2 stars (if_minus_plus)  *)
-(** Prove the following hoare triple using [hoare_if]: *)
-
-Theorem if_minus_plus :
-  {{fun st => True}}
-  IFB (BLe (AId X) (AId Y))
-    THEN (Z ::= AMinus (AId Y) (AId X))
-    ELSE (Y ::= APlus (AId X) (AId Z))
-  FI
-  {{fun st => st Y = st X + st Z}}.
-Proof.
-  (* FILL IN HERE *) Admitted.
-
-(* ----------------------------------------------------------------- *)
-(** *** Exercise: One-sided conditionals *)
-
-(** **** Exercise: 4 stars (if1_hoare)  *)
-
-(** In this exercise we consider extending Imp with "one-sided
-    conditionals" of the form [IF1 b THEN c FI]. Here [b] is a
-    boolean expression, and [c] is a command. If [b] evaluates to
-    [true], then command [c] is evaluated. If [b] evaluates to
-    [false], then [IF1 b THEN c FI] does nothing.
-
-    We recommend that you do this exercise before the ones that
-    follow, as it should help solidify your understanding of the
-    material. *)
-
-(** The first step is to extend the syntax of commands and introduce
-    the usual notations.  (We've done this for you.  We use a separate
-    module to prevent polluting the global name space.) *)
-
-Module If1.
-
-Inductive com : Type :=
-  | CSkip : com
-  | CAss : id -> aexp -> com
-  | CSeq : com -> com -> com
-  | CIf : bexp -> com -> com -> com
-  | CWhile : bexp -> com -> com
-  | CIf1 : bexp -> com -> com.
-
-Notation "'SKIP'" :=
-  CSkip.
-Notation "c1 ;; c2" :=
-  (CSeq c1 c2) (at level 80, right associativity).
-Notation "X '::=' a" :=
-  (CAss X a) (at level 60).
-Notation "'WHILE' b 'DO' c 'END'" :=
-  (CWhile b c) (at level 80, right associativity).
-Notation "'IFB' e1 'THEN' e2 'ELSE' e3 'FI'" :=
-  (CIf e1 e2 e3) (at level 80, right associativity).
-Notation "'IF1' b 'THEN' c 'FI'" :=
-  (CIf1 b c) (at level 80, right associativity).
-
-(** Next we need to extend the evaluation relation to accommodate
-    [IF1] branches.  This is for you to do... What rule(s) need to be
-    added to [ceval] to evaluate one-sided conditionals? *)
-
-Reserved Notation "c1 '/' st '\\' st'" (at level 40, st at level 39).
-
-Inductive ceval : com -> state -> state -> Prop :=
-  | E_Skip : forall st : state, SKIP / st \\ st
-  | E_Ass : forall (st : state) (a1 : aexp) (n : nat) (X : id),
-            aeval st a1 = n -> (X ::= a1) / st \\ t_update st X n
-  | E_Seq : forall (c1 c2 : com) (st st' st'' : state),
-            c1 / st \\ st' -> c2 / st' \\ st'' -> (c1 ;; c2) / st \\ st''
-  | E_IfTrue : forall (st st' : state) (b1 : bexp) (c1 c2 : com),
-               beval st b1 = true ->
-               c1 / st \\ st' -> (IFB b1 THEN c1 ELSE c2 FI) / st \\ st'
-  | E_IfFalse : forall (st st' : state) (b1 : bexp) (c1 c2 : com),
-                beval st b1 = false ->
-                c2 / st \\ st' -> (IFB b1 THEN c1 ELSE c2 FI) / st \\ st'
-  | E_WhileEnd : forall (b1 : bexp) (st : state) (c1 : com),
-                 beval st b1 = false -> (WHILE b1 DO c1 END) / st \\ st
-  | E_WhileLoop : forall (st st' st'' : state) (b1 : bexp) (c1 : com),
-                  beval st b1 = true ->
-                  c1 / st \\ st' ->
-                  (WHILE b1 DO c1 END) / st' \\ st'' ->
-                  (WHILE b1 DO c1 END) / st \\ st''
-(* FILL IN HERE *)
-
-  where "c1 '/' st '\\' st'" := (ceval c1 st st').
-
-(** Now we repeat (verbatim) the definition and notation of Hoare triples. *)
-
-Definition hoare_triple (P:Assertion) (c:com) (Q:Assertion) : Prop :=
-  forall st st',
-       c / st \\ st'  ->
-       P st  ->
-       Q st'.
-
-Notation "{{ P }}  c  {{ Q }}" := (hoare_triple P c Q)
-                                  (at level 90, c at next level)
-                                  : hoare_spec_scope.
-
-(** Finally, we (i.e., you) need to state and prove a theorem,
-    [hoare_if1], that expresses an appropriate Hoare logic proof rule
-    for one-sided conditionals. Try to come up with a rule that is
-    both sound and as precise as possible. *)
-
-(* FILL IN HERE *)
-
-(** For full credit, prove formally [hoare_if1_good] that your rule is
-    precise enough to show the following valid Hoare triple:
-
-  {{ X + Y = Z }}
-  IF1 Y <> 0 THEN
-    X ::= X + Y
-  FI
-  {{ X = Z }}
-*)
-
-(** Hint: Your proof of this triple may need to use the other proof
-    rules also. Because we're working in a separate module, you'll
-    need to copy here the rules you find necessary. *)
-
-Lemma hoare_if1_good :
-  {{ fun st => st X + st Y = st Z }}
-  IF1 BNot (BEq (AId Y) (ANum 0)) THEN
-    X ::= APlus (AId X) (AId Y)
-  FI
-  {{ fun st => st X = st Z }}.
-Proof. (* FILL IN HERE *) Admitted.
-
-End If1.
-(** [] *)
-
-(* ================================================================= *)
 (** ** Loops *)
 
-(** Finally, we need a rule for reasoning about while loops. *)
-
-(** Suppose we have a loop
-
-      WHILE b DO c END
-
-    and we want to find a pre-condition [P] and a post-condition
-    [Q] such that
-
-      {{P}} WHILE b DO c END {{Q}}
-
-    is a valid triple. *)
-
-(** First of all, let's think about the case where [b] is false at the
-    beginning -- i.e., let's assume that the loop body never executes
-    at all.  In this case, the loop behaves like [SKIP], so we might
-    be tempted to write: *)
-
-(**
-
-      {{P}} WHILE b DO c END {{P}}.
-*)
-
-(** But, as we remarked above for the conditional, we know a
-    little more at the end -- not just [P], but also the fact
-    that [b] is false in the current state.  So we can enrich the
-    postcondition a little: *)
-(**
-
-      {{P}} WHILE b DO c END {{P /\ ~b}}
-*)
-
-(** What about the case where the loop body _does_ get executed?
-    In order to ensure that [P] holds when the loop finally
-    exits, we certainly need to make sure that the command [c]
-    guarantees that [P] holds whenever [c] is finished.
-    Moreover, since [P] holds at the beginning of the first
-    execution of [c], and since each execution of [c]
-    re-establishes [P] when it finishes, we can always assume
-    that [P] holds at the beginning of [c].  This leads us to the
-    following rule: *)
-(**
-
-                   {{P}} c {{P}}
-        -----------------------------------
-        {{P}} WHILE b DO c END {{P /\ ~b}}
-*)
-(** This is almost the rule we want, but again it can be improved a
-    little: at the beginning of the loop body, we know not only that
-    [P] holds, but also that the guard [b] is true in the current
-    state.  This gives us a little more information to use in
-    reasoning about [c] (showing that it establishes the invariant by
-    the time it finishes).  This gives us the final version of the
-    rule:
-*)
 (**
 
                {{P /\ b}} c {{P}}
@@ -779,10 +241,10 @@ End If1.
 *)
 
 Lemma hoare_while : forall P b c,
-  {{fun st => P st /\ bassn b st}} c {{P}} ->
-  {{P}} WHILE b DO c END {{fun st => P st /\ ~ (bassn b st)}}.
+  {{fun h v => P h v /\ bassn b h v}} c {{P}} ->
+  {{P}} WHILE b DO c END {{fun h v => P h v /\ ~ (bassn b h v)}}.
 Proof.
-  intros P b c Hhoare st st' He HP.
+  intros P b c Hhoare h h' v v' He HP.
   (* Like we've seen before, we need to reason by induction
      on [He], because, in the "keep looping" case, its hypotheses
      talk about the whole loop instead of just [c]. *)
@@ -793,202 +255,40 @@ Proof.
     split. assumption. apply bexp_eval_false. assumption.
   - (* E_WhileLoop *)
     apply IHHe2. reflexivity.
-    apply (Hhoare st st'). assumption.
+    unfold hoare_triple in Hhoare.
+    apply (Hhoare h1 h2 v1 v2). assumption.
       split. assumption. apply bexp_eval_true. assumption.
 Qed.
 
-(** One subtlety in the terminology is that calling some assertion [P]
-    a "loop invariant" doesn't just mean that it is preserved by the
-    body of the loop in question (i.e., [{{P}} c {{P}}], where [c] is
-    the loop body), but rather that [P] _together with the fact that
-    the loop's guard is true_ is a sufficient precondition for [c] to
-    ensure [P] as a postcondition.
+(* ================================================================= *)
+(** ** Memory write *)
 
-    This is a slightly (but significantly) weaker requirement.  For
-    example, if [P] is the assertion [X = 0], then [P] _is_ an
-    invariant of the loop
+(**
 
-    WHILE X = 2 DO X := 1 END
+      ------------------------------ (hoare_heap_write)
+      {{Q [X |-> a]}} X **= a {{Q}}
+ *)
 
-    although it is clearly _not_ preserved by the body of the
-    loop. *)
+Definition heap_sub a1 a2 P : Assertion :=
+  fun (h : heap) (v : valuation) =>
+    P (t_update h (Id (aeval h v a1)) (aeval h v a2)) v.
 
-Example while_example :
-    {{fun st => st X <= 3}}
-  WHILE (BLe (AId X) (ANum 2))
-  DO X ::= APlus (AId X) (ANum 1) END
-    {{fun st => st X = 3}}.
+Notation "P [ '[' a1 ']' |-> a2 ]" := (heap_sub a1 a2 P) (at level 10).
+
+Theorem hoare_heap_write : forall Q a1 a2,
+  {{Q [ [a1] |-> a2]}} (a1 **= a2) {{Q}}.
 Proof.
-  eapply hoare_consequence_post.
-  apply hoare_while.
-  eapply hoare_consequence_pre.
-  apply hoare_asgn.
-  unfold bassn, assn_sub, assert_implies, t_update. simpl.
-    intros st [H1 H2]. apply leb_complete in H2. omega.
-  unfold bassn, assert_implies. intros st [Hle Hb].
-    simpl in Hb. destruct (leb (st X) 2) eqn : Heqle.
-    exfalso. apply Hb; reflexivity.
-    apply leb_iff_conv in Heqle. omega.
-Qed.
+  unfold hoare_triple.
+  intros.
+  inversion H. subst.
+  unfold heap_sub in H0. apply H0.  Qed.
 
-(** We can use the while rule to prove the following Hoare triple,
-    which may seem surprising at first... *)
 
-Theorem always_loop_hoare : forall P Q,
-  {{P}} WHILE BTrue DO SKIP END {{Q}}.
-Proof.
-  (* WORKED IN CLASS *)
-  intros P Q.
-  apply hoare_consequence_pre with (P' := fun st : state => True).
-  eapply hoare_consequence_post.
-  apply hoare_while.
-  - (* Loop body preserves invariant *)
-    apply hoare_post_true. intros st. apply I.
-  - (* Loop invariant and negated guard imply postcondition *)
-    simpl. intros st [Hinv Hguard].
-    exfalso. apply Hguard. reflexivity.
-  - (* Precondition implies invariant *)
-    intros st H. constructor.  Qed.
-
-(** Of course, this result is not surprising if we remember that
-    the definition of [hoare_triple] asserts that the postcondition
-    must hold _only_ when the command terminates.  If the command
-    doesn't terminate, we can prove anything we like about the
-    post-condition. *)
-
-(** Hoare rules that only talk about terminating commands are
-    often said to describe a logic of "partial" correctness.  It is
-    also possible to give Hoare rules for "total" correctness, which
-    build in the fact that the commands terminate. However, in this
-    course we will only talk about partial correctness. *)
-
-(* ----------------------------------------------------------------- *)
-(** *** Exercise: [REPEAT] *)
-
-(** **** Exercise: 4 stars, advanced (hoare_repeat)  *)
-(** In this exercise, we'll add a new command to our language of
-    commands: [REPEAT] c [UNTIL] a [END]. You will write the
-    evaluation rule for [repeat] and add a new Hoare rule to
-    the language for programs involving it. *)
-
-Module RepeatExercise.
-
-Inductive com : Type :=
-  | CSkip : com
-  | CAsgn : id -> aexp -> com
-  | CSeq : com -> com -> com
-  | CIf : bexp -> com -> com -> com
-  | CWhile : bexp -> com -> com
-  | CRepeat : com -> bexp -> com.
-
-(** [REPEAT] behaves like [WHILE], except that the loop guard is
-    checked _after_ each execution of the body, with the loop
-    repeating as long as the guard stays _false_.  Because of this,
-    the body will always execute at least once. *)
-
-Notation "'SKIP'" :=
-  CSkip.
-Notation "c1 ;; c2" :=
-  (CSeq c1 c2) (at level 80, right associativity).
-Notation "X '::=' a" :=
-  (CAsgn X a) (at level 60).
-Notation "'WHILE' b 'DO' c 'END'" :=
-  (CWhile b c) (at level 80, right associativity).
-Notation "'IFB' e1 'THEN' e2 'ELSE' e3 'FI'" :=
-  (CIf e1 e2 e3) (at level 80, right associativity).
-Notation "'REPEAT' e1 'UNTIL' b2 'END'" :=
-  (CRepeat e1 b2) (at level 80, right associativity).
-
-(** Add new rules for [REPEAT] to [ceval] below.  You can use the rules
-    for [WHILE] as a guide, but remember that the body of a [REPEAT]
-    should always execute at least once, and that the loop ends when
-    the guard becomes true.  Then update the [ceval_cases] tactic to
-    handle these added cases.  *)
-
-Inductive ceval : state -> com -> state -> Prop :=
-  | E_Skip : forall st,
-      ceval st SKIP st
-  | E_Ass  : forall st a1 n X,
-      aeval st a1 = n ->
-      ceval st (X ::= a1) (t_update st X n)
-  | E_Seq : forall c1 c2 st st' st'',
-      ceval st c1 st' ->
-      ceval st' c2 st'' ->
-      ceval st (c1 ;; c2) st''
-  | E_IfTrue : forall st st' b1 c1 c2,
-      beval st b1 = true ->
-      ceval st c1 st' ->
-      ceval st (IFB b1 THEN c1 ELSE c2 FI) st'
-  | E_IfFalse : forall st st' b1 c1 c2,
-      beval st b1 = false ->
-      ceval st c2 st' ->
-      ceval st (IFB b1 THEN c1 ELSE c2 FI) st'
-  | E_WhileEnd : forall b1 st c1,
-      beval st b1 = false ->
-      ceval st (WHILE b1 DO c1 END) st
-  | E_WhileLoop : forall st st' st'' b1 c1,
-      beval st b1 = true ->
-      ceval st c1 st' ->
-      ceval st' (WHILE b1 DO c1 END) st'' ->
-      ceval st (WHILE b1 DO c1 END) st''
-(* FILL IN HERE *)
-.
-
-(** A couple of definitions from above, copied here so they use the
-    new [ceval]. *)
-
-Notation "c1 '/' st '\\' st'" := (ceval st c1 st')
-                                 (at level 40, st at level 39).
-
-Definition hoare_triple (P:Assertion) (c:com) (Q:Assertion)
-                        : Prop :=
-  forall st st', (c / st \\ st') -> P st -> Q st'.
-
-Notation "{{ P }}  c  {{ Q }}" :=
-  (hoare_triple P c Q) (at level 90, c at next level).
-
-(** To make sure you've got the evaluation rules for [REPEAT] right,
-    prove that [ex1_repeat evaluates correctly. *)
-
-Definition ex1_repeat :=
-  REPEAT
-    X ::= ANum 1;;
-    Y ::= APlus (AId Y) (ANum 1)
-  UNTIL (BEq (AId X) (ANum 1)) END.
-
-Theorem ex1_repeat_works :
-  ex1_repeat / empty_state \\
-               t_update (t_update empty_state X 1) Y 1.
-Proof.
-  (* FILL IN HERE *) Admitted.
-
-(** Now state and prove a theorem, [hoare_repeat], that expresses an
-    appropriate proof rule for [repeat] commands.  Use [hoare_while]
-    as a model, and try to make your rule as precise as possible. *)
-
-(* FILL IN HERE *)
-
-(** For full credit, make sure (informally) that your rule can be used
-    to prove the following valid Hoare triple:
-
-  {{ X > 0 }}
-  REPEAT
-    Y ::= X;;
-    X ::= X - 1
-  UNTIL X = 0 END
-  {{ X = 0 /\ Y > 0 }}
-*)
-
-End RepeatExercise.
-(** [] *)
 
 (* ################################################################# *)
 (** * Summary *)
 
-(** So far, we've introduced Hoare Logic as a tool for reasoning about
-    Imp programs.  In the reminder of this chapter we'll explore a
-    systematic way to use Hoare Logic to prove properties about
-    programs. The rules of Hoare Logic are:
+(** The rules of Hoare Logic are:
 
              ------------------------------ (hoare_asgn)
              {{Q [X |-> a]}} X::=a {{Q}}
@@ -1016,92 +316,14 @@ End RepeatExercise.
          -----------------------------   (hoare_consequence)
                 {{P}} c {{Q}}
 
-    In the next chapter, we'll see how these rules are used to prove
-    that programs satisfy specifications of their behavior. *)
+
+             ------------------------------ (hoare_heap_write)
+             {{Q [X |-> a]}} X**=a {{Q}}
+
+
+ *)
 
 (* ################################################################# *)
-(** * Additional Exercises *)
-
-(** **** Exercise: 3 stars (himp_hoare)  *)
-(** In this exercise, we will derive proof rules for the [HAVOC]
-    command, which we studied in the last chapter.
-
-    First, we enclose this work in a separate module, and recall the
-    syntax and big-step semantics of Himp commands. *)
-
-Module Himp.
-
-Inductive com : Type :=
-  | CSkip : com
-  | CAsgn : id -> aexp -> com
-  | CSeq : com -> com -> com
-  | CIf : bexp -> com -> com -> com
-  | CWhile : bexp -> com -> com
-  | CHavoc : id -> com.
-
-Notation "'SKIP'" :=
-  CSkip.
-Notation "X '::=' a" :=
-  (CAsgn X a) (at level 60).
-Notation "c1 ;; c2" :=
-  (CSeq c1 c2) (at level 80, right associativity).
-Notation "'WHILE' b 'DO' c 'END'" :=
-  (CWhile b c) (at level 80, right associativity).
-Notation "'IFB' e1 'THEN' e2 'ELSE' e3 'FI'" :=
-  (CIf e1 e2 e3) (at level 80, right associativity).
-Notation "'HAVOC' X" := (CHavoc X) (at level 60).
-
-Reserved Notation "c1 '/' st '\\' st'" (at level 40, st at level 39).
-
-Inductive ceval : com -> state -> state -> Prop :=
-  | E_Skip : forall st : state, SKIP / st \\ st
-  | E_Ass : forall (st : state) (a1 : aexp) (n : nat) (X : id),
-            aeval st a1 = n -> (X ::= a1) / st \\ t_update st X n
-  | E_Seq : forall (c1 c2 : com) (st st' st'' : state),
-            c1 / st \\ st' -> c2 / st' \\ st'' -> (c1 ;; c2) / st \\ st''
-  | E_IfTrue : forall (st st' : state) (b1 : bexp) (c1 c2 : com),
-               beval st b1 = true ->
-               c1 / st \\ st' -> (IFB b1 THEN c1 ELSE c2 FI) / st \\ st'
-  | E_IfFalse : forall (st st' : state) (b1 : bexp) (c1 c2 : com),
-                beval st b1 = false ->
-                c2 / st \\ st' -> (IFB b1 THEN c1 ELSE c2 FI) / st \\ st'
-  | E_WhileEnd : forall (b1 : bexp) (st : state) (c1 : com),
-                 beval st b1 = false -> (WHILE b1 DO c1 END) / st \\ st
-  | E_WhileLoop : forall (st st' st'' : state) (b1 : bexp) (c1 : com),
-                  beval st b1 = true ->
-                  c1 / st \\ st' ->
-                  (WHILE b1 DO c1 END) / st' \\ st'' ->
-                  (WHILE b1 DO c1 END) / st \\ st''
-  | E_Havoc : forall (st : state) (X : id) (n : nat),
-              (HAVOC X) / st \\ t_update st X n
-
-  where "c1 '/' st '\\' st'" := (ceval c1 st st').
-
-(** The definition of Hoare triples is exactly as before. Unlike our
-    notion of program equivalence, which had subtle consequences with
-    occassionally nonterminating commands (exercise [havoc_diverge]),
-    this definition is still fully satisfactory. Convince yourself of
-    this before proceeding. *)
-
-Definition hoare_triple (P:Assertion) (c:com) (Q:Assertion) : Prop :=
-  forall st st', c / st \\ st' -> P st -> Q st'.
-
-Notation "{{ P }}  c  {{ Q }}" := (hoare_triple P c Q)
-                                  (at level 90, c at next level)
-                                  : hoare_spec_scope.
-
-(** Complete the Hoare rule for [HAVOC] commands below by defining
-    [havoc_pre] and prove that the resulting rule is correct. *)
-
-Definition havoc_pre (X : id) (Q : Assertion) : Assertion 
-  (* REPLACE THIS LINE WITH   := _your_definition_ . *) . Admitted.
-
-Theorem hoare_havoc : forall (Q : Assertion) (X : id),
-  {{ havoc_pre X Q }} HAVOC X {{ Q }}.
-Proof.
-  (* FILL IN HERE *) Admitted.
-
-End Himp.
 (** [] *)
 
 (** $Date: 2016-07-13 12:41:41 -0400 (Wed, 13 Jul 2016) $ *)
